more proofs and more refinement

Weidenbach_Book/IsaSAT/IsaSAT_Arena.thy
@@ -2197,4 +2197,127 @@ lemma mop_arena_update_lit_spec:
   subgoal using assms by (auto intro!: valid_arena_arenap_update_lit)
   done
 
+definition arena_set_status where
+  \<open>arena_set_status arena C b= do {
+    (arena[C - STATUS_SHIFT := AStatus b (arena_used arena C) (arena_lbd arena C)])
+  }\<close>
+
+lemma length_arena_set_status[simp]:
+  \<open>length (arena_set_status arena C b) = length arena\<close>
+  by (auto simp: arena_set_status_def)
+
+lemma header_size_Suc_def:
+  \<open>header_size C =
+    (if is_short_clause C then (Suc (Suc 0)) else (Suc (Suc (Suc 0))))\<close>
+  unfolding header_size_def
+  by auto
+
+lemma valid_arena_arena_set_status:
+  assumes
+    valid: \<open>valid_arena arena N vdm\<close> and
+    C: \<open>C \<in># dom_m N\<close> and
+    b: \<open>b = IRRED \<or> b = LEARNED\<close> and
+    b': \<open>b' \<longleftrightarrow> b = IRRED\<close>
+  shows \<open>valid_arena (arena_set_status arena C b) (fmupd C (N \<propto> C, b') N) vdm\<close>
+proof -
+  have [simp]: \<open>i - 2 \<le> length arena\<close> and
+    [simp]: \<open>C - 2 = i - 2 \<longleftrightarrow> C =i\<close> if \<open>i \<in> vdm\<close> for i
+    apply (meson less_imp_diff_less less_imp_le_nat that valid valid_arena_def)
+    by (metis C STATUS_SHIFT_def add_diff_inverse_nat arena_lifting(16) that valid valid_arena_in_vdom_le_arena(2) verit_comp_simplify1(3))
+  have [iff]: \<open>arena_dead_clause (Misc.slice (i - 2) i (arena_set_status arena C b)) \<longleftrightarrow>
+    arena_dead_clause (Misc.slice (i - 2) i arena)\<close>
+    if \<open>i \<notin># dom_m N\<close> and \<open>i \<in> vdm\<close> for i
+    using minimal_difference_between_invalid_index2[OF valid C that(1) _ that(2)]
+      minimal_difference_between_invalid_index[OF valid C that(1) _ that(2)]
+      that
+    by (cases \<open>i < C\<close>)
+      (auto simp: extra_information_mark_to_delete_def drop_update_swap
+      arena_dead_clause_def SHIFTS_def arena_set_status_def ac_simps nth_list_update' nth_drop
+       Misc.slice_def header_size_def split: if_splits)
+
+  have [simp]: \<open>header_size (N \<propto> C) - POS_SHIFT < C + length (N \<propto> C) - (C - header_size (N \<propto> C))\<close>
+     \<open>header_size (N \<propto> C) - STATUS_SHIFT < C + length (N \<propto> C) - (C - header_size (N \<propto> C))\<close>
+     \<open>header_size (N \<propto> C) - SIZE_SHIFT < C + length (N \<propto> C) - (C - header_size (N \<propto> C))\<close>
+    apply (smt (verit, ccfv_threshold) C add.right_neutral add_diff_inverse_nat diff_is_0_eq' le_zero_eq
+      length_greater_0_conv less_diff_conv less_imp_diff_less list.size(3) nat.simps(3)
+      nat_add_left_cancel_less numeral_2_eq_2 valid valid_arena_def xarena_active_clause_alt_def)
+    apply (smt (verit, ccfv_SIG) C Nat.diff_add_assoc2 STATUS_SHIFT_def arena_lifting(1)
+      arena_shift_distinct(16) diff_diff_cancel diff_is_0_eq nat.simps(3) nat_le_linear
+      not_add_less1 not_gr0 numeral_2_eq_2 valid zero_less_diff)
+      using C SIZE_SHIFT_def arena_lifting(1) valid verit_comp_simplify1(3) by fastforce
+
+  have [iff]: \<open>C - header_size (N \<propto> C) \<le> length arena\<close>
+    by (meson C arena_lifting(2) less_imp_diff_less less_imp_le_nat valid)
+  have  \<open>C \<ge> header_size (N \<propto> C)\<close> \<open>C < length arena\<close>
+    using arena_lifting[OF valid C] by auto
+  then have [iff]: \<open>C - LBD_SHIFT < length arena\<close>
+     \<open>C - SIZE_SHIFT < length arena\<close>
+    \<open>is_long_clause (N \<propto> C) \<Longrightarrow> header_size (N \<propto> C) \<ge> POS_SHIFT\<close> and
+    [simp]: \<open>C - header_size (N \<propto> C) + header_size (N \<propto> C) = C\<close>
+    by (auto simp: LBD_SHIFT_def SIZE_SHIFT_def header_size_def POS_SHIFT_def split: if_splits)
+
+
+  have [simp]: \<open>C - header_size (N \<propto> C) + (header_size (N \<propto> C) - LBD_SHIFT) = C - LBD_SHIFT\<close>
+    \<open>C - header_size (N \<propto> C) + (header_size (N \<propto> C) - SIZE_SHIFT) = C - SIZE_SHIFT\<close>
+    \<open>is_long_clause (N \<propto> C) \<Longrightarrow> C - header_size (N \<propto> C) + header_size (N \<propto> C) - POS_SHIFT = C - POS_SHIFT\<close>
+    apply (smt (verit, best) C Nat.add_diff_assoc2 add.right_neutral add_diff_cancel_right
+      add_diff_inverse_nat arena_lifting(1) arena_shift_distinct(16) diff_is_0_eq' less_imp_le_nat
+      order_mono_setup.refl valid)
+    apply (metis Nat.diff_add_assoc One_nat_def SIZE_SHIFT_def STATUS_SHIFT_def \<open>header_size (N \<propto> C) \<le> C\<close>
+      arena_shift_distinct(10) diff_is_0_eq le_add_diff_inverse2 lessI less_or_eq_imp_le nat_le_linear numeral_2_eq_2)
+    using SHIFTS_alt_def(1) header_size_def by presburger
+  have [iff]: \<open>C - LBD_SHIFT = C - SIZE_SHIFT \<longleftrightarrow> False\<close>
+    \<open>is_long_clause (N \<propto> C) \<Longrightarrow> C - LBD_SHIFT = C - POS_SHIFT \<longleftrightarrow> False\<close>
+    \<open>C - LBD_SHIFT < C\<close>
+    apply (metis \<open>header_size (N \<propto> C) \<le> C\<close> arena_shift_distinct(10))
+    using \<open>header_size (N \<propto> C) \<le> C\<close> arena_shift_distinct(13) apply presburger
+    by (metis STATUS_SHIFT_def \<open>header_size (N \<propto> C) \<le> C\<close> diff_less header_size_Suc_def le_zero_eq nat.simps(3) not_gr0 numeral_2_eq_2)
+
+  let ?s = \<open>clause_slice (arena_set_status arena C b) N C\<close>
+  let ?t = \<open>clause_slice arena N C\<close>
+  have [simp]: \<open>is_Pos (?s ! (header_size (N \<propto> C) - POS_SHIFT)) = is_Pos (?t ! (header_size (N \<propto> C) - POS_SHIFT))\<close>
+    \<open>is_Status (?s ! (header_size (N \<propto> C) - STATUS_SHIFT))\<close>
+    \<open>xarena_status (?s ! (header_size (N \<propto> C) - LBD_SHIFT)) = b\<close>
+    \<open>is_Size (?s ! (header_size (N \<propto> C) - SIZE_SHIFT)) = is_Size (?t ! (header_size (N \<propto> C) - SIZE_SHIFT))\<close>
+    \<open>xarena_length (?s ! (header_size (N \<propto> C) - SIZE_SHIFT)) = xarena_length (?t ! (header_size (N \<propto> C) - SIZE_SHIFT))\<close>
+    \<open>is_long_clause (N \<propto> C) \<Longrightarrow> xarena_pos (?s ! (header_size (N \<propto> C) - POS_SHIFT)) = xarena_pos (?t ! (header_size (N \<propto> C) - POS_SHIFT))\<close>
+    \<open>length ?s = length ?t\<close>
+    \<open>Misc.slice C (C + length (N \<propto> C)) (arena_set_status arena C b) = Misc.slice C (C + length (N \<propto> C)) arena\<close>
+    apply (auto simp: arena_set_status_def Misc.slice_def nth_list_update')
+    apply (metis C arena_el.distinct_disc(11) arena_lifting(14) valid)
+    done
+  have \<open>xarena_active_clause (clause_slice arena N C) (the (fmlookup N C))\<close>
+    using assms(1,2) unfolding valid_arena_def by (auto dest!: multi_member_split)
+  then have [simp]: \<open>xarena_active_clause (clause_slice (arena_set_status arena C b) N C) (N \<propto> C, b')\<close>
+    using b' b unfolding xarena_active_clause_def case_prod_beta
+    by (auto simp: xarena_active_clause_def)
+  have [simp]: \<open>(clause_slice (arena_set_status arena C b) N i) = (clause_slice arena N i)\<close>
+    if \<open>C \<noteq> i\<close> and \<open>i \<in># dom_m N\<close> for i
+    using 
+      valid_minimal_difference_between_valid_index[OF valid that(2) C]
+      valid_minimal_difference_between_valid_index[OF valid C that(2)]
+      that
+    apply (cases \<open>C > i\<close>)
+    apply (auto simp: Misc.slice_def arena_set_status_def)
+    apply (subst drop_update_swap)
+    using \<open>C - header_size (N \<propto> C) + (header_size (N \<propto> C) - LBD_SHIFT) = C - LBD_SHIFT\<close> apply linarith
+    apply (subst take_update_cancel)
+    using \<open>C - header_size (N \<propto> C) + (header_size (N \<propto> C) - LBD_SHIFT) = C - LBD_SHIFT\<close> apply linarith
+    apply auto
+    apply (subst drop_upd_irrelevant)
+    using \<open>C - LBD_SHIFT < C\<close> apply linarith
+    apply auto
+    done
+
+  show ?thesis
+    using assms(1,2)
+    unfolding valid_arena_def
+    by auto
+qed
+
+definition mop_arena_set_status where
+  \<open>mop_arena_set_status arena C b= do {
+    ASSERT(arena_is_valid_clause_idx arena C);
+    RETURN(arena_set_status arena C b)
+  }\<close>
 end
