Weidenbach_Book/IsaSAT/IsaSAT_Simplify_Forward_Subsumption_LLVM.thy
@@ -4,10 +4,158 @@ theory IsaSAT_Simplify_Forward_Subsumption_LLVM
     IsaSAT_Setup_LLVM
     IsaSAT_Trail_LLVM
     IsaSAT_Proofs_LLVM
+    IsaSAT_Arena_Sorting_LLVM
 begin
 
 no_notation WB_More_Refinement.fref (\<open>[_]\<^sub>f _ \<rightarrow> _\<close> [0,60,60] 60)
 no_notation WB_More_Refinement.freft (\<open>_ \<rightarrow>\<^sub>f _\<close> [60,60] 60)
+
+definition clause_size_sort_clauses_raw :: \<open>arena \<Rightarrow> vdom \<Rightarrow> nat \<Rightarrow> nat \<Rightarrow> nat list nres\<close> where
+  \<open>clause_size_sort_clauses_raw arena N = pslice_sort_spec idx_clause_cdom clause_size_less arena N\<close>
+
+definition clause_size_sort_clauses_avdom :: \<open>arena \<Rightarrow> vdom \<Rightarrow> nat list nres\<close> where
+  \<open>clause_size_sort_clauses_avdom arena N = clause_size_sort_clauses_raw arena N 0 (length N)\<close>
+
+lemmas Size_Ordering_introsort[sepref_fr_rules] =
+  Size_Ordering_it.introsort_param_impl_correct[unfolded clause_size_sort_clauses_raw_def[symmetric] PR_CONST_def]
+
+sepref_register clause_size_sort_clauses_raw
+sepref_def clause_size_sort_clauses_avdom_impl
+  is \<open>uncurry clause_size_sort_clauses_avdom\<close>
+  :: \<open>arena_fast_assn\<^sup>k *\<^sub>a vdom_fast_assn\<^sup>d \<rightarrow>\<^sub>a vdom_fast_assn\<close>
+  supply[[goals_limit=1]]
+  unfolding clause_size_sort_clauses_avdom_def
+  apply (annot_snat_const \<open>TYPE(64)\<close>)
+  by sepref
+
+definition clause_size_sort_clauses :: \<open>arena \<Rightarrow> aivdom2 \<Rightarrow> aivdom2 nres\<close> where
+  \<open>clause_size_sort_clauses arena N = map_tvdom_aivdom_int (clause_size_sort_clauses_avdom arena) N\<close>
+
+sepref_def clause_size_sort_clauses_impl
+  is \<open>uncurry clause_size_sort_clauses\<close>
+  :: \<open>arena_fast_assn\<^sup>k *\<^sub>a aivdom_int_assn\<^sup>d \<rightarrow>\<^sub>a aivdom_int_assn\<close>
+  unfolding clause_size_sort_clauses_def map_tvdom_aivdom_int_def
+  by sepref
+
+lemma
+  map_vdom_aivdom_int2:
+  \<open>(uncurry (\<lambda>arena. map_vdom_aivdom_int (f arena)), uncurry (\<lambda>arena. map_vdom_aivdom (f arena)))
+  \<in> Id \<times>\<^sub>r aivdom_rel \<rightarrow>\<^sub>f \<langle>aivdom_rel\<rangle>nres_rel\<close>
+  apply (intro frefI nres_relI)
+  subgoal for x y
+    using map_vdom_aivdom_int[of \<open>f (fst x)\<close>]
+    apply (cases x; cases y)
+    apply (auto intro!: frefI nres_relI simp: fref_def nres_rel_def)
+    done
+  done
+
+lemma get_aivdom_eq_aivdom_iff:
+  \<open>IsaSAT_VDom.get_aivdom b = (x1, a, aa, ba) \<longleftrightarrow> b = AIvdom (x1, a, aa, ba)\<close>
+  by (cases b) auto
+hide_const (open) NEMonad.ASSERT NEMonad.RETURN NEMonad.ASSERT NEMonad.SPEC
+
+definition sort_cands_by_length2 :: \<open>_ \<Rightarrow> isasat_aivdom \<Rightarrow> isasat_aivdom nres\<close> where
+  \<open>sort_cands_by_length2 arena avdom = do {
+  ASSERT (\<forall>i\<in>set (get_tvdom_aivdom avdom). arena_is_valid_clause_idx arena i);
+  SPEC (\<lambda>cands'.
+       mset (get_tvdom_aivdom cands') = mset (get_tvdom_aivdom avdom) \<and>
+       (get_avdom_aivdom cands') = (get_avdom_aivdom avdom) \<and>
+       (get_ivdom_aivdom cands') = (get_ivdom_aivdom avdom) \<and>
+       (get_vdom_aivdom cands') = (get_vdom_aivdom avdom) \<and>
+    sorted_wrt (\<lambda>a b. arena_length arena a \<le> arena_length arena b) (get_tvdom_aivdom cands'))
+}\<close>
+
+lemma quicksort_clauses_by_score_sort:
+  \<open>(uncurry clause_size_sort_clauses, uncurry sort_cands_by_length2) \<in>
+  Id \<times>\<^sub>r aivdom_rel \<rightarrow>\<^sub>f \<langle>aivdom_rel\<rangle>nres_rel\<close>
+  apply (intro fun_relI nres_relI frefI)
+  subgoal for arena arena'
+    unfolding uncurry_def sort_cands_by_length2_def map_tvdom_aivdom_int_def
+      clause_size_sort_clauses_def clause_size_sort_clauses_avdom_def
+      clause_size_sort_clauses_raw_def pslice_sort_spec_def nres_monad3
+    apply (refine_vcg)
+    subgoal for x1 x2 x1a x2a x1b x2b x1c x2c
+      by (cases x2) (auto simp: idx_clause_cdom_def code_hider_rel_def)
+    subgoal for x1 x2 x1a x2a x1b x2b x1c x2c
+      apply (rule specify_left)
+      apply (rule order_trans)
+      apply (rule slice_sort_spec_refine_sort)
+      apply (auto simp:
+        pslice_sort_spec_def le_ASSERT_iff idx_cdom_def slice_rel_def br_def uncurry_def
+        conc_fun_RES sort_spec_def map_vdom_aivdom_int_def 
+        code_hider_rel_def
+        split:prod.splits
+        simp del: slice_complete
+        intro!: ASSERT_leI 
+        )
+      subgoal for x1d x
+        using slice_complete[of x]
+        apply (rule_tac x = \<open>AIvdom (x1d, x1b, x1c, x)\<close> in exI)
+        apply (case_tac x2; auto simp: clause_size_less_def slice_complete
+          le_by_lt_def)
+        unfolding le_by_lt_def
+        apply (auto simp: clause_size_less_def
+          intro!: arg_cong[of \<open>(\<lambda>a b. \<not> arena_length x1 b < arena_length x1 a)\<close> \<open>(\<lambda>a b. arena_length x1 a \<le> arena_length x1 b)\<close> \<open>\<lambda>a. sorted_wrt a x\<close>, THEN iffD1]ext
+          )
+        done
+      done
+    done
+  done
+
+
+
+context
+  notes [fcomp_norm_unfold] = aivdom_assn_alt_def[symmetric] aivdom_assn_def[symmetric]
+begin
+
+lemma clause_size_sort_clauses_impl_sort_cands_by_length2[sepref_fr_rules]:
+  \<open>(uncurry clause_size_sort_clauses_impl, uncurry sort_cands_by_length2)
+  \<in> (al_assn arena_el_impl_assn)\<^sup>k *\<^sub>a aivdom_assn\<^sup>d \<rightarrow>\<^sub>a aivdom_assn\<close>
+  (is \<open>?c \<in> [?pre]\<^sub>a ?im \<rightarrow> ?f\<close>)
+proof -
+  have H: \<open>?c
+\<in> [comp_PRE (Id \<times>\<^sub>f aivdom_rel) (\<lambda>_. True) (\<lambda>x y. True)
+   (\<lambda>x. nofail (uncurry sort_cands_by_length2 x))]\<^sub>a ?im \<rightarrow> ?f\<close>
+    (is \<open>_ \<in> [?pre']\<^sub>a ?im' \<rightarrow> _\<close>)
+    using hfref_compI_PRE[OF clause_size_sort_clauses_impl.refine,
+  OF quicksort_clauses_by_score_sort[unfolded convert_fref], unfolded fcomp_norm_unfold] by blast
+  have pre: \<open>?pre' x\<close> if \<open>?pre x\<close> for x
+    using that 
+    by (case_tac x, case_tac \<open>snd x\<close>)
+      (auto simp: comp_PRE_def code_hider_rel_def)
+  show ?thesis
+    apply (rule hfref_weaken_pre[OF ])
+     defer
+    using H apply assumption
+    using pre ..
+qed
+
+end
+
+
+lemma sort_cands_by_length_alt_def:
+  \<open>sort_cands_by_length S\<^sub>0 = do {
+  let (aivdom, S) = extract_vdom_wl_heur S\<^sub>0;
+  ASSERT (aivdom = get_aivdom S\<^sub>0);
+  let (arena, S) = extract_arena_wl_heur S;
+  ASSERT (arena = get_clauses_wl_heur S\<^sub>0);
+  aivdom \<leftarrow> sort_cands_by_length2 arena aivdom;
+  let S = update_arena_wl_heur arena S;
+  let S = update_vdom_wl_heur aivdom S;
+  RETURN S
+}\<close>
+    apply (auto simp: sort_cands_by_length_def sort_cands_by_length2_def state_extractors Let_def RES_RETURN_RES image_iff
+      intro!: bind_cong[OF refl]
+         split: isasat_int_splits)
+    apply (case_tac xb)
+    apply auto
+    done
+
+sepref_def sort_cands_by_length_impl
+  is sort_cands_by_length
+  :: \<open>isasat_bounded_assn\<^sup>d \<rightarrow>\<^sub>a isasat_bounded_assn\<close>
+  unfolding sort_cands_by_length_alt_def
+  by sepref
 
 (*TODO: kill mop_arena_lit2_st*)
 sepref_def isa_all_lit_clause_unset
@@ -41,7 +189,7 @@ lemma rdomp_isasat_bounded_assn_length_avdomD:
 
 
 sepref_register isa_all_lit_clause_unset isa_push_to_occs_list_st
-  find_best_subsumption_candidate 
+  find_best_subsumption_candidate sort_cands_by_length
 
 sepref_def find_best_subsumption_candidate_code
   is \<open>uncurry find_best_subsumption_candidate\<close>
@@ -124,9 +272,8 @@ sepref_def push_to_tvdom_st_impl
   unfolding push_to_tvdom_st_alt_def isasat_fast_relaxed_def
   by sepref
 
-sepref_register isa_good_candidate_for_subsumption sort_cands_by_length
+sepref_register isa_good_candidate_for_subsumption
 
-term sort_cands_by_length
 lemma isa_populate_occs_inv_isasat_fast_relaxedI:
   \<open>isa_populate_occs_inv x cands (a1', a2') \<Longrightarrow> isasat_fast_relaxed x \<Longrightarrow> isasat_fast_relaxed a2'\<close>
   by (auto simp: isa_populate_occs_inv_def isasat_fast_relaxed_def)
@@ -141,22 +288,410 @@ sepref_def isa_populate_occs_code
     al_fold_custom_empty[where 'l=64] Let_def[of \<open>get_avdom _\<close>] Let_def[of \<open>get_occs _\<close>]
     Let_def[of \<open>get_tvdom _\<close>]
   apply (annot_snat_const \<open>TYPE(64)\<close>)
+  by sepref
+
+sepref_register isa_forward_subsumption_all_wl2 isa_populate_occs
+
+sepref_register isa_forward_subsumption_all mop_cch_create mop_cch_add_all_clause
+  mop_cch_add mop_cch_in
+
+
+abbreviation cch_assn where
+  \<open>cch_assn \<equiv> IICF_Array.array_assn bool1_assn\<close>
+
+sepref_def mop_cch_create_impl
+  is mop_cch_create
+  :: \<open>sint64_nat_assn\<^sup>k \<rightarrow>\<^sub>a cch_assn\<close>
+  unfolding mop_cch_create_def  op_list_replicate_def[symmetric] array_fold_custom_replicate
+  by sepref
+
+sepref_def mop_cch_add_impl
+  is \<open>uncurry mop_cch_add\<close>
+  :: \<open>unat_lit_assn\<^sup>k *\<^sub>a cch_assn\<^sup>d \<rightarrow>\<^sub>a cch_assn\<close>
+  unfolding mop_cch_add_def cch_add_def cch_add_pre_def
+  by sepref
+
+
+sepref_def mop_cch_in_impl
+  is \<open>uncurry mop_cch_in\<close>
+  :: \<open>unat_lit_assn\<^sup>k *\<^sub>a cch_assn\<^sup>k \<rightarrow>\<^sub>a bool1_assn\<close>
+  unfolding mop_cch_in_def cch_in_def cch_in_pre_def
+  by sepref
+
+sepref_def mop_cch_add_all_clause_impl
+  is \<open>uncurry2 mop_cch_add_all_clause\<close>
+  :: \<open>isasat_bounded_assn\<^sup>k *\<^sub>a sint64_nat_assn\<^sup>k *\<^sub>a cch_assn\<^sup>d \<rightarrow>\<^sub>a cch_assn\<close>
+  unfolding mop_cch_add_all_clause_def
+    mop_access_lit_in_clauses_heur_def[symmetric]
+  supply [dest] = isasat_bounded_assn_length_arenaD
+  supply [[goals_limit=1]]
+  apply (annot_snat_const \<open>TYPE(64)\<close>)
+  by sepref
+
+
+
+sepref_register isa_try_to_forward_subsume_wl2
+
+
+sepref_def isa_try_to_forward_subsume_wl2_break_impl
+  is isa_try_to_forward_subsume_wl2_break
+  :: \<open>isasat_bounded_assn\<^sup>k \<rightarrow>\<^sub>a bool1_assn\<close>
+  unfolding isa_try_to_forward_subsume_wl2_break_def
+  by sepref
+
+sepref_register isa_try_to_forward_subsume_wl2_break
+
+(*TODO requiring anything from the unused parts of the struct is not really useful*)
+definition subsumption_rel :: \<open>('c \<times> nat) set
+  \<Rightarrow> ('b \<times> 'd literal) set \<Rightarrow> ('c \<times> nat) set \<Rightarrow> ((3 word \<times> 'b \<times> _) \<times> 'd subsumption) set\<close> where
+subsumption_rel_internal_def:  \<open>subsumption_rel R1 R2 R3 = {((tag, x, y),b).
+  case b of NONE \<Rightarrow> tag = 0
+          | SUBSUMED_BY x' \<Rightarrow> (y, x') \<in> R1 \<and> tag = 1
+          | STRENGTHENED_BY x' y' \<Rightarrow> (x, x') \<in> R2 \<and> (y, y') \<in> R3 \<and> tag = 2}\<close>
+
+lemma subsumption_rel_def: \<open>\<langle>R1,R2,R3\<rangle>subsumption_rel = {((tag, x, y),b).
+  case b of NONE \<Rightarrow> tag = 0
+          | SUBSUMED_BY x' \<Rightarrow> (y, x') \<in> R1 \<and> tag = 1
+    | STRENGTHENED_BY x' y' \<Rightarrow> (x, x') \<in> R2 \<and> (y, y') \<in> R3 \<and> tag = 2}\<close>
+    unfolding subsumption_rel_internal_def relAPP_def by auto
+
+definition is_NONE where
+  \<open>is_NONE x \<longleftrightarrow> NONE = x\<close>
+lemma is_subsumption:
+  \<open>(\<lambda>(tag, _). tag = 0, is_NONE) \<in> \<langle>R1,R2,R3\<rangle>subsumption_rel \<rightarrow> bool_rel\<close>
+  \<open>(\<lambda>(tag, _). tag = 1, is_subsumed) \<in> \<langle>R1,R2,R3\<rangle>subsumption_rel \<rightarrow> bool_rel\<close>
+  \<open>(\<lambda>(tag, _). tag = 2, is_strengthened) \<in> \<langle>R1,R2,R3\<rangle>subsumption_rel \<rightarrow> bool_rel\<close>
+  \<open>((0, 0, 0), NONE) \<in> \<langle>R1,R2,R3\<rangle>subsumption_rel\<close>
+  \<open>(\<lambda>C. (1, 0, C), SUBSUMED_BY) \<in> R1 \<rightarrow> \<langle>R1,R2,R3\<rangle>subsumption_rel\<close>
+  \<open>(\<lambda>C D. (2, C, D), STRENGTHENED_BY) \<in> R2 \<rightarrow> R3 \<rightarrow> \<langle>R1,R2,R3\<rangle>subsumption_rel\<close>
+  \<open>(\<lambda>(tag, C, D). D, subsumed_by) \<in> [is_subsumed]\<^sub>f \<langle>R1,R2,R3\<rangle>subsumption_rel \<rightarrow> R1\<close>
+  \<open>(\<lambda>(tag, C, D). D, strengthened_by) \<in> [is_strengthened]\<^sub>f \<langle>R1,R2,R3\<rangle>subsumption_rel \<rightarrow> R3\<close>
+  \<open>(\<lambda>(tag, C, D). C, strengthened_on_lit) \<in> [is_strengthened]\<^sub>f \<langle>R1,R2,R3\<rangle>subsumption_rel \<rightarrow> R2\<close>
+  unfolding subsumption_rel_def
+  by (auto simp: IS_LEFT_UNIQUE_def single_valued_def is_NONE_def
+    intro!: frefI
+    split: subsumption.splits)
+
+abbreviation subsumption_raw_assn where
+  \<open>subsumption_raw_assn \<equiv> word_assn' TYPE(3) \<times>\<^sub>a word_assn \<times>\<^sub>a id_assn\<close>
+
+definition subsumption_assn where
+  \<open>subsumption_assn = hr_comp subsumption_raw_assn (\<langle>snat_rel' TYPE(64), unat_lit_rel,snat_rel' TYPE(64)\<rangle>subsumption_rel)\<close>
+
+
+sepref_definition is_NONE_impl
+  is \<open>RETURN o (\<lambda>(tag, _). tag = 0)\<close>
+  :: \<open>subsumption_raw_assn\<^sup>k \<rightarrow>\<^sub>a bool1_assn\<close>
+  by sepref
+
+sepref_definition is_subsumed_impl
+  is \<open>RETURN o (\<lambda>(tag, _). tag = 1)\<close>
+  :: \<open>subsumption_raw_assn\<^sup>k \<rightarrow>\<^sub>a bool1_assn\<close>
+  by sepref
+
+
+sepref_definition is_strengthened_impl
+  is \<open>RETURN o (\<lambda>(tag, _). tag = 2)\<close>
+  :: \<open>subsumption_raw_assn\<^sup>k \<rightarrow>\<^sub>a bool1_assn\<close>
+  by sepref
+
+sepref_definition STRENGTHENED_BY_impl
+  is \<open>uncurry (RETURN oo (\<lambda>C D. (2, C, D)))\<close>
+  :: \<open>word_assn\<^sup>k *\<^sub>a id_assn\<^sup>k \<rightarrow>\<^sub>a subsumption_raw_assn\<close>
+  by sepref
+
+sepref_definition SUBSUMED_BY_impl
+  is \<open>RETURN o (\<lambda>C. (1, 0, C))\<close>
+  :: \<open>word_assn\<^sup>k \<rightarrow>\<^sub>a subsumption_raw_assn\<close>
+  by sepref
+
+sepref_definition NONE_impl
+  is \<open>uncurry0 (RETURN (0, 0, 0::64 word))\<close>
+  :: \<open>unit_assn\<^sup>k \<rightarrow>\<^sub>a subsumption_raw_assn\<close>
+  by sepref
+
+sepref_definition subsumed_by_impl
+  is \<open>RETURN o (\<lambda>(tag, C, D). D)\<close>
+  :: \<open>subsumption_raw_assn\<^sup>k \<rightarrow>\<^sub>a id_assn\<close>
+  by sepref
+
+sepref_definition strengthened_on_lit_impl
+  is \<open>RETURN o (\<lambda>(tag, C, D). C)\<close>
+  :: \<open>subsumption_raw_assn\<^sup>k \<rightarrow>\<^sub>a word_assn\<close>
+  by sepref
+
+sepref_register is_NONE is_subsumed is_strengthened STRENGTHENED_BY SUBSUMED_BY NONE subsumed_by strengthened_by strengthened_on_lit
+
+lemmas [sepref_fr_rules] = 
+  is_NONE_impl.refine[FCOMP is_subsumption(1), of \<open>snat_rel' TYPE(64)\<close> \<open>unat_lit_rel\<close> \<open>snat_rel' TYPE(64)\<close>, unfolded subsumption_assn_def[symmetric] is_NONE_def[symmetric]]
+  is_subsumed_impl.refine[FCOMP is_subsumption(2), of \<open>snat_rel' TYPE(64)\<close> \<open>unat_lit_rel\<close> \<open>snat_rel' TYPE(64)\<close>, unfolded subsumption_assn_def[symmetric]]
+  is_strengthened_impl.refine[FCOMP is_subsumption(3), of \<open>snat_rel' TYPE(64)\<close> \<open>unat_lit_rel\<close> \<open>snat_rel' TYPE(64)\<close>, unfolded subsumption_assn_def[symmetric]]
+  SUBSUMED_BY_impl.refine[FCOMP is_subsumption(5), of \<open>snat_assn' TYPE(64)\<close> unat_lit_rel \<open>snat_rel' TYPE(64)\<close>, unfolded the_pure_pure subsumption_assn_def[symmetric]]
+  STRENGTHENED_BY_impl.refine[FCOMP is_subsumption(6), of unat_lit_assn \<open>snat_assn' TYPE(64)\<close> \<open>snat_rel' TYPE(64)\<close>, unfolded the_pure_pure subsumption_assn_def[symmetric]]
+  NONE_impl.refine[FCOMP is_subsumption(4), of \<open>snat_rel' TYPE(64)\<close> unat_lit_rel \<open>snat_rel' TYPE(64)\<close>, unfolded the_pure_pure subsumption_assn_def[symmetric]]
+  subsumed_by_impl.refine[FCOMP is_subsumption(7), of \<open>snat_assn' TYPE(64)\<close> unat_lit_rel \<open>snat_rel' TYPE(64)\<close>, unfolded the_pure_pure subsumption_assn_def[symmetric]]
+  subsumed_by_impl.refine[FCOMP is_subsumption(8), of \<open>snat_assn' TYPE(64)\<close> \<open>snat_rel' TYPE(64)\<close> unat_lit_rel, unfolded the_pure_pure subsumption_assn_def[symmetric]]
+  strengthened_on_lit_impl.refine[FCOMP is_subsumption(9), of unat_lit_assn \<open>snat_rel' TYPE(64)\<close> \<open>snat_rel' TYPE(64)\<close>, unfolded the_pure_pure subsumption_assn_def[symmetric]]
+
+lemma fold_is_NONE: \<open>x = NONE \<longleftrightarrow> is_NONE x\<close> \<open>NONE = x \<longleftrightarrow> is_NONE x\<close>
+  by (auto simp: is_NONE_def)
+
+lemma isa_subsume_clauses_match2_alt_def:
+  \<open>isa_subsume_clauses_match2 C' C N D = do {
+  ASSERT (isa_subsume_clauses_match2_pre C' C N D);
+  n \<leftarrow> mop_arena_length_st N C';
+  ASSERT (n < Suc (uint32_max div 2));
+  (i, st) \<leftarrow> WHILE\<^sub>T\<^bsup> \<lambda>(i,s). True\<^esup> (\<lambda>(i, st). i < n\<and> st \<noteq> NONE)
+    (\<lambda>(i, st). do {
+      ASSERT (i < n);
+      L \<leftarrow> mop_arena_lit2 (get_clauses_wl_heur N) C' i;
+      lin \<leftarrow> mop_cch_in L D;
+      if lin
+      then RETURN (i+1, st)
+      else do {
+      lin \<leftarrow> mop_cch_in (-L) D;
+      if lin
+      then if is_subsumed st
+      then do {mop_free st; RETURN (i+1, STRENGTHENED_BY L C')}
+      else do {mop_free st; RETURN (i+1, NONE)}
+      else do {mop_free st; RETURN (i+1, NONE)}
+    }})
+     (0, SUBSUMED_BY C');
+  RETURN st
+        }\<close>
+   unfolding isa_subsume_clauses_match2_def sorry
+
+schematic_goal mk_free_lbd_assn[sepref_frame_free_rules]: \<open>MK_FREE subsumption_assn ?fr\<close>
+  unfolding subsumption_assn_def by synthesize_free+
+
+
+lemma [safe_constraint_rules]: \<open>CONSTRAINT is_pure subsumption_assn\<close>
+  unfolding subsumption_assn_def by auto
+
+sepref_register isa_subsume_clauses_match2 
+sepref_def isa_subsume_clauses_match2_impl
+  is \<open>uncurry3 isa_subsume_clauses_match2\<close>
+  :: \<open>sint64_nat_assn\<^sup>k *\<^sub>a sint64_nat_assn\<^sup>k *\<^sub>a  isasat_bounded_assn\<^sup>k *\<^sub>a cch_assn\<^sup>k \<rightarrow>\<^sub>a subsumption_assn\<close>
+  unfolding isa_subsume_clauses_match2_alt_def fold_is_NONE
+    mop_access_lit_in_clauses_heur_def[symmetric]
+  apply (annot_snat_const \<open>TYPE(64)\<close>)
+  by sepref
+
+sepref_def mop_cch_remove_one_impl
+  is \<open>uncurry mop_cch_remove_one\<close>
+  :: \<open>unat_lit_assn\<^sup>k *\<^sub>a cch_assn\<^sup>d \<rightarrow>\<^sub>a cch_assn\<close>
+  unfolding mop_cch_remove_one_def
+  by sepref
+
+sepref_register mop_cch_remove_one mop_arena_status_st mop_arena_promote_st
+
+(*TODO share with propagation!*)
+sepref_def swap_lits_impl is \<open>uncurry3 mop_arena_swap\<close>
+  :: \<open>sint64_nat_assn\<^sup>k *\<^sub>a sint64_nat_assn\<^sup>k *\<^sub>a sint64_nat_assn\<^sup>k *\<^sub>a arena_fast_assn\<^sup>d \<rightarrow>\<^sub>a arena_fast_assn\<close>
+  unfolding mop_arena_swap_def swap_lits_pre_def
+  unfolding gen_swap
+  by sepref
+
+sepref_def mop_cch_remove_all_clauses_impl
+  is \<open>uncurry2 mop_cch_remove_all_clauses\<close>
+  :: \<open>isasat_bounded_assn\<^sup>k *\<^sub>a sint64_nat_assn\<^sup>k *\<^sub>a cch_assn\<^sup>d \<rightarrow>\<^sub>a cch_assn\<close>
+  unfolding mop_cch_remove_all_clauses_def mop_access_lit_in_clauses_heur_def[symmetric]
+    mop_arena_length_st_def[symmetric]
+  supply [dest] = isasat_bounded_assn_length_arenaD
+  apply (annot_snat_const \<open>TYPE(64)\<close>)
+  by sepref
+
+sepref_register ASize
+
+lemma arena_is_valid_clause_idxD:
+  assumes \<open>arena_is_valid_clause_idx a b\<close>
+    \<open>rdomp (al_assn arena_el_impl_assn) a\<close>
+    \<open>j \<le> arena_length a b\<close>
+  shows \<open>j - 2  < max_unat 32\<close>
+proof -
+  obtain N vdom where
+    \<open>valid_arena a N vdom\<close> and
+    \<open>b \<in># dom_m N\<close>
+    using assms(1) unfolding arena_is_valid_clause_idx_def
+    by auto
+  then have eq: \<open>length (N \<propto> b) = arena_length a b\<close> and
+    le: \<open>b < length a\<close> and
+    size: \<open>is_Size (a ! (b - SIZE_SHIFT))\<close>
+    by (auto simp: arena_lifting)
+
+  have \<open>i<length a \<Longrightarrow> rdomp arena_el_impl_assn (a ! i)\<close> for i
+    using rdomp_al_dest'[OF assms(2)]
+    by auto
+  from this[of \<open>b - SIZE_SHIFT\<close>] have \<open>rdomp arena_el_impl_assn (a ! (b - SIZE_SHIFT))\<close>
+    using le by auto
+  then have \<open>length (N \<propto> b) \<le> uint32_max + 2\<close>
+    using size eq unfolding rdomp_pure
+    apply (auto simp: rdomp_def arena_el_impl_rel_def is_Size_def
+       comp_def pure_def unat_rel_def unat.rel_def br_def arena_el_rel_def
+       arena_length_def uint32_max_def)
+     subgoal for x
+       using unat_lt_max_unat[of x]
+       apply (auto simp: max_unat_def)
+       done
+    done
+  then show ?thesis
+    using assms POS_SHIFT_def
+    unfolding isa_update_pos_pre_def
+    by (auto simp: arena_is_valid_clause_idx_def arena_lifting eq
+       uint32_max_def max_unat_def)
+qed
+
+lemma arena_is_valid_clause_idxD2: \<open>arena_is_valid_clause_idx b a \<Longrightarrow> a - Suc 0 < length b\<close>
+  \<open>arena_is_valid_clause_idx b a \<Longrightarrow> MAX_LENGTH_SHORT_CLAUSE < arena_length b a \<Longrightarrow> 3 \<le> a\<close>
+  \<open>arena_is_valid_clause_idx b a \<Longrightarrow> MAX_LENGTH_SHORT_CLAUSE < arena_length b a \<Longrightarrow> a - 3 < length b\<close>
+  using arena_lengthI(2) less_imp_diff_less apply blast
+  apply (auto simp: arena_is_valid_clause_idx_def header_size_def arena_lifting split: if_splits dest: arena_lifting(1)[of _ _ _ a])
+  apply (metis arena_header_size_def arena_lifting(1) valid_arena_header_size)
+  using valid_arena_def by fastforce
+
+sepref_def mop_arena_shorten_impl
+  is \<open>uncurry2 mop_arena_shorten\<close>
+  :: \<open>sint64_nat_assn\<^sup>k  *\<^sub>a sint64_nat_assn\<^sup>k *\<^sub>a arena_fast_assn\<^sup>d \<rightarrow>\<^sub>a arena_fast_assn\<close>
+  unfolding mop_arena_shorten_def arena_shorten_def arena_shorten_pre_def SIZE_SHIFT_def POS_SHIFT_def
+    arena_is_valid_clause_idxD2
+  supply [intro] = arena_lengthI arena_is_valid_clause_idxD arena_is_valid_clause_idxD2
+  apply (rewrite at \<open>APos \<hole>\<close> unat_const_fold[where 'a=32])
+  apply (annot_snat_const \<open>TYPE(64)\<close>)
+  apply (rewrite at \<open>If _ (_[_ := ASize \<hole>, _ := _]) _\<close> annot_snat_unat_downcast[where 'l=32])
+  apply (rewrite at \<open>If _ _ (_[_ := ASize \<hole>])\<close> annot_snat_unat_downcast[where 'l=32])
+  by sepref
+
+sepref_def remove_lit_from_clause_impl
+  is \<open>uncurry2 remove_lit_from_clause\<close>
+  :: \<open>arena_fast_assn\<^sup>d *\<^sub>a sint64_nat_assn\<^sup>k *\<^sub>a unat_lit_assn\<^sup>k \<rightarrow>\<^sub>a arena_fast_assn\<close>
+  unfolding remove_lit_from_clause_def if_not_swap
+  apply (annot_snat_const \<open>TYPE(64)\<close>)
+  by sepref
+
+lemma remove_lit_from_clause_st_alt_def: \<open>remove_lit_from_clause_st S C L = do {
+    let (N, S) = extract_arena_wl_heur S;
+    N \<leftarrow> remove_lit_from_clause N C L;
+    RETURN (update_arena_wl_heur N S)
+}\<close>
+  by (auto simp: remove_lit_from_clause_st_def state_extractors push_to_tvdom_st_def
+         split: isasat_int_splits)
+
+sepref_def remove_lit_from_clause_st_impl
+  is \<open>uncurry2 remove_lit_from_clause_st\<close>
+  :: \<open>isasat_bounded_assn\<^sup>d *\<^sub>a sint64_nat_assn\<^sup>k *\<^sub>a unat_lit_assn\<^sup>k \<rightarrow>\<^sub>a isasat_bounded_assn\<close>
+  unfolding remove_lit_from_clause_st_alt_def
+  by sepref
+
+sepref_register remove_lit_from_clause_st
+
+lemma mark_garbage_heur_as_subsumed_alt_def:
+  \<open>mark_garbage_heur_as_subsumed C S\<^sub>0 = (do{
+    ASSERT (arena_is_valid_clause_vdom (get_clauses_wl_heur S\<^sub>0) C);
+    ASSERT (mark_garbage_pre (get_clauses_wl_heur S\<^sub>0, C));
+    size \<leftarrow> mop_arena_length (get_clauses_wl_heur S\<^sub>0) C;
+    let (N', S) = extract_arena_wl_heur S\<^sub>0;
+    ASSERT (N' = get_clauses_wl_heur S\<^sub>0);
+    let st = arena_status N' C = IRRED;
+    let N' = extra_information_mark_to_delete (N') C;
+    let (lcount, S) = extract_lcount_wl_heur S;
+    ASSERT(\<not>st \<longrightarrow> clss_size_lcount lcount \<ge> 1);
+    let lcount = (if st then lcount else (clss_size_decr_lcount lcount));
+    let (stats, S) = extract_stats_wl_heur S;
+    let stats = (if st then decr_irred_clss stats else stats);
+    let S = update_arena_wl_heur N' S;
+    let S = update_lcount_wl_heur lcount S;
+    let S = update_stats_wl_heur stats S;
+    let S = incr_wasted_st (of_nat size) S;
+    RETURN S
+  })\<close>
+      by (auto simp: mark_garbage_heur_as_subsumed_def Let_def state_extractors push_to_tvdom_st_def
+        intro!: bind_cong[OF refl]
+         split: isasat_int_splits)
+
+sepref_def mark_garbage_heur_as_subsumed_impl
+  is \<open>uncurry mark_garbage_heur_as_subsumed\<close>
+  :: \<open>sint64_nat_assn\<^sup>k *\<^sub>a isasat_bounded_assn\<^sup>d \<rightarrow>\<^sub>a isasat_bounded_assn\<close>
+  supply [[goals_limit=1]]
+  supply of_nat_snat[sepref_import_param]
+  unfolding mark_garbage_heur_as_subsumed_alt_def
+    mop_arena_length_st_def[symmetric]
+  by sepref
+
+sepref_def isa_strengthen_clause_wl2_impl
+  is \<open>uncurry3 isa_strengthen_clause_wl2\<close>
+  :: \<open>sint64_nat_assn\<^sup>k *\<^sub>a sint64_nat_assn\<^sup>k *\<^sub>a unat_lit_assn\<^sup>k *\<^sub>a isasat_bounded_assn\<^sup>d \<rightarrow>\<^sub>a isasat_bounded_assn\<close>
+  unfolding isa_strengthen_clause_wl2_def mop_arena_status_st_def[symmetric]
+    mop_arena_length_st_def[symmetric]
+  by sepref
+
+  
+lemma subsumption_cases_split:
+  \<open>(case s of SUBSUMED_BY s \<Rightarrow> f s | STRENGTHENED_BY x y \<Rightarrow> g x y | NONE \<Rightarrow> h) =
+  (if is_NONE s then h else if is_subsumed s then f (subsumed_by s) else do {ASSERT (is_strengthened s); g (strengthened_on_lit s) (strengthened_by s)})\<close>
+  by (auto simp: is_NONE_def split: subsumption.splits)
+
+sepref_register isa_strengthen_clause_wl2 isa_subsume_or_strengthen_wl
+sepref_def isa_subsume_or_strengthen_wl_impl
+  is \<open>uncurry2 isa_subsume_or_strengthen_wl\<close>
+  :: \<open>sint64_nat_assn\<^sup>k *\<^sub>a subsumption_assn\<^sup>k *\<^sub>a isasat_bounded_assn\<^sup>d \<rightarrow>\<^sub>a isasat_bounded_assn\<close>
+  unfolding isa_subsume_or_strengthen_wl_def subsumption_cases_split mop_arena_status_st_def[symmetric]
+  by sepref
+
+sepref_def isa_forward_subsumption_one_wl_impl
+  is \<open>uncurry3 isa_forward_subsumption_one_wl\<close>
+  :: \<open>[\<lambda>((_, _), S). isasat_fast_relaxed S]\<^sub>asint64_nat_assn\<^sup>k *\<^sub>a  cch_assn\<^sup>d *\<^sub>a unat_lit_assn\<^sup>k *\<^sub>a isasat_bounded_assn\<^sup>d \<rightarrow> isasat_bounded_assn \<times>\<^sub>a bool1_assn \<times>\<^sub>a cch_assn\<close>
+  supply [dest] = rdomp_isasat_bounded_assn_length_avdomD isasat_bounded_assn_length_arenaD
+  supply [[goals_limit=1]]
+  unfolding isa_forward_subsumption_one_wl_def get_occs_list_at_def[symmetric] fold_is_NONE
+    mop_access_lit_in_clauses_heur_def[symmetric] length_occs_at_def[symmetric] mop_arena_status_st_def[symmetric]
+  apply (annot_snat_const \<open>TYPE(64)\<close>)
+  by sepref
+
+lemma isa_try_to_forward_subsume_wl_invI:
+  \<open>isa_try_to_forward_subsume_wl_inv S C (i, changed, break, D, T)\<Longrightarrow> isasat_fast_relaxed S \<Longrightarrow> isasat_fast_relaxed T\<close>
+  unfolding isa_try_to_forward_subsume_wl_inv_def prod.simps
+apply normalize_goal+
+apply (auto simp add: isasat_fast_relaxed_def)
+sorry
+
+
+
+sepref_def isa_try_to_forward_subsume_wl2_impl
+  is \<open>uncurry2 isa_try_to_forward_subsume_wl2\<close>
+  :: \<open>[\<lambda>((_, _), S). isasat_fast_relaxed S]\<^sub>a sint64_nat_assn\<^sup>k *\<^sub>a  cch_assn\<^sup>d *\<^sub>a isasat_bounded_assn\<^sup>d \<rightarrow> cch_assn \<times>\<^sub>a isasat_bounded_assn\<close>
+  unfolding isa_try_to_forward_subsume_wl2_def
+    mop_access_lit_in_clauses_heur_def[symmetric]
+  supply [[goals_limit=1]]
+  supply [intro] = isa_try_to_forward_subsume_wl_invI
+  apply (annot_snat_const \<open>TYPE(64)\<close>)
   apply sepref_dbg_keep
   apply sepref_dbg_trans_keep
   apply sepref_dbg_trans_step_keep
   apply sepref_dbg_side_unfold
-  subgoal premises p
-apply auto
-  oops
+subgoal premises p
+using p(5-9,30-34)
+apply (auto simp: max_snat_def uint32_max_def)
+oops
 
-thm isa_populate_occs_def
-thm access_avdom_at_def
-find_theorems get_avdom length
-thm isa_forward_subsumption_all_wl2_def
-sepref_register isa_forward_subsumption_all_wl2 isa_populate_occs
 
-sepref_register isa_forward_subsumption_all
 
+end
+term isa_try_to_forward_subsume_wl2
+
+sepref_def isa_forward_subsumption_all_wl2_impl
+  is isa_forward_subsumption_all_wl2
+  :: \<open>[isasat_fast_relaxed]\<^sub>a isasat_bounded_assn\<^sup>d \<rightarrow> isasat_bounded_assn\<close>
+  unfolding isa_forward_subsumption_all_wl2_def
+    access_tvdom_at_def[symmetric] length_tvdom_def[symmetric]
+    length_watchlist_raw_def[symmetric]
+  apply (annot_snat_const \<open>TYPE(64)\<close>)
+  apply sepref_dbg_keep
+  apply sepref_dbg_trans_keep
+  apply sepref_dbg_trans_step_keep
+  apply sepref_dbg_side_unfold
+subgoal premises p
+oops
+  
 sepref_def isa_forward_subsumption_all
   is \<open>isa_forward_subsumption_all\<close>
   :: \<open>isasat_bounded_assn\<^sup>d \<rightarrow>\<^sub>a isasat_bounded_assn\<close>
